theories/case_studies/cmdc/cmdc_spec.v
@@ -1,7 +1,8 @@
 From iris.proofmode Require Import proofmode.
 From cap_machine Require Import region_invariants_allocation region_invariants_revocation interp_weakening.
-From cap_machine Require Import logrel logrel_extra rules proofmode.
+From cap_machine Require Import logrel logrel_extra rules.
 From cap_machine Require Import fetch assert switcher_spec_call cmdc.
+From cap_machine Require Import proofmode.
 
 Section CMDC.
   Context
