theories/case_studies/counter/counter_spec.v
@@ -1,8 +1,9 @@
 From iris.proofmode Require Import proofmode.
 From cap_machine Require Import region_invariants_allocation region_invariants_revocation interp_weakening.
-From cap_machine Require Import logrel logrel_extra rules proofmode.
+From cap_machine Require Import logrel logrel_extra rules.
 From cap_machine Require Import fetch switcher_spec_call counter.
 From cap_machine Require Import switcher_spec_return.
+From cap_machine Require Import proofmode.
 
 Section Counter.
   Context
