theories/case_studies/vae/vae_spec_closure.v
@@ -1,8 +1,9 @@
 From iris.proofmode Require Import proofmode.
 From cap_machine Require Import region_invariants_allocation region_invariants_revocation interp_weakening monotone.
 From cap_machine Require Import rules logrel logrel_extra monotone proofmode register_tactics.
-From cap_machine Require Import fetch assert interp_switcher_call switcher_spec_call switcher_spec_call_alt switcher_spec_return.
+From cap_machine Require Import fetch assert switcher interp_switcher_call switcher_spec_call switcher_spec_call_alt switcher_spec_return.
 From cap_machine Require Import vae vae_helper.
+From cap_machine Require Import proofmode.
 
 Section VAE.
   Context
@@ -268,7 +269,7 @@ Section VAE.
     ∗ inv (export_table_PCCN VAEN) (b_vae_exp_tbl ↦ₐ WCap RX Global pc_b pc_e pc_b)
     ∗ inv (export_table_CGPN VAEN) ((b_vae_exp_tbl ^+ 1)%a ↦ₐ WCap RW Global cgp_b cgp_e cgp_b)
     ∗ inv (export_table_entryN VAEN (b_vae_exp_tbl ^+ 2)%a)
-        ((b_vae_exp_tbl ^+ 2)%a ↦ₐ WInt (switcher.encode_entry_point 1 (length (imports ++ VAE_main_code_init))))
+        ((b_vae_exp_tbl ^+ 2)%a ↦ₐ WInt (encode_entry_point 1 (length (imports ++ VAE_main_code_init))))
     ∗ WSealed ot_switcher (SCap RO g_vae_exp_tbl b_vae_exp_tbl e_vae_exp_tbl (b_vae_exp_tbl ^+ 2)%a)
         ↦□ₑ 1
     ∗ seal_pred ot_switcher ot_switcher_propC
@@ -1106,7 +1107,7 @@ Section VAE.
     ∗ inv (export_table_PCCN VAEN) (b_vae_exp_tbl ↦ₐ WCap RX Global pc_b pc_e pc_b)
     ∗ inv (export_table_CGPN VAEN) ((b_vae_exp_tbl ^+ 1)%a ↦ₐ WCap RW Global cgp_b cgp_e cgp_b)
     ∗ inv (export_table_entryN VAEN (b_vae_exp_tbl ^+ 2)%a)
-        ((b_vae_exp_tbl ^+ 2)%a ↦ₐ WInt (switcher.encode_entry_point 1 (length (imports ++ VAE_main_code_init))))
+        ((b_vae_exp_tbl ^+ 2)%a ↦ₐ WInt (encode_entry_point 1 (length (imports ++ VAE_main_code_init))))
     ∗ WSealed ot_switcher (SCap RO Global b_vae_exp_tbl e_vae_exp_tbl (b_vae_exp_tbl ^+ 2)%a)
         ↦□ₑ 1
     ∗ WSealed ot_switcher (SCap RO Local b_vae_exp_tbl e_vae_exp_tbl (b_vae_exp_tbl ^+ 2)%a)
