theories/logrel/ftlr/JmpCap.v
@@ -14,7 +14,6 @@ Section fundamental.
     {stsg : STSG Addr region_type Σ} {cstackg : CSTACKG Σ} {heapg : heapGS Σ}
     {nainv: logrel_na_invs Σ}
     `{MP: MachineParameters}
-    {swlayout : switcherLayout}
   .
 
   Implicit Types W : WORLD.
@@ -29,12 +28,12 @@ Section fundamental.
 
   Lemma jmpcap_case (W : WORLD) (C : CmptName) (regs : leibnizO Reg)
     (p p': Perm) (g : Locality) (b e a : Addr)
-    (w : Word) (ρ : region_type) (rsrc : RegName) (P:V) (cstk : CSTK) (Ws : list WORLD) (Cs : list CmptName) (wstk : Word) (Nswitcher : namespace) :
-    ftlr_instr W C regs p p' g b e a w (JmpCap rsrc) ρ P cstk Ws Cs wstk Nswitcher.
+    (w : Word) (ρ : region_type) (rsrc : RegName) (P:V) (cstk : CSTK) (Ws : list WORLD) (Cs : list CmptName) (wstk : Word) :
+    ftlr_instr W C regs p p' g b e a w (JmpCap rsrc) ρ P cstk Ws Cs wstk.
   Proof.
     intros Hp Hsome HcorrectPC Hbae Hfp HO Hpers Hpwl Hregion Hnotrevoked Hi.
     iIntros "#IH #Hinv_interp #Hreg #Hinva #Hrcond #Hwcond #Hmono #HmonoV Hw Hcont %Hframe Hsts Hown Hcstk".
-    iIntros "Hr Hstate Ha HPC Hmap %Hwstk #Hinv_switcher".
+    iIntros "Hr Hstate Ha HPC Hmap %Hwstk".
     destruct (decide (rsrc = PC)) as [HrPC|HrPC].
     - subst rsrc.
       iApply (wp_jmpcap_successPC with "[HPC Ha]"); eauto; first iFrame.
