theories/logrel/fundamental.v
@@ -7,7 +7,6 @@ From iris.proofmode Require Import proofmode.
 From iris.program_logic Require Import weakestpre adequacy lifting.
 From stdpp Require Import base.
 From cap_machine Require Export logrel register_tactics.
-From cap_machine Require Export switcher_preamble.
 
 Section fundamental.
   Context
@@ -17,7 +16,6 @@ Section fundamental.
     {stsg : STSG Addr region_type Σ} {cstackg : CSTACKG Σ} {heapg : heapGS Σ}
     {nainv: logrel_na_invs Σ}
     `{MP: MachineParameters}
-    {swlayout : switcherLayout}
   .
 
   Implicit Types W : WORLD.
@@ -33,12 +31,11 @@ Section fundamental.
   Theorem fundamental_cap
     (W : WORLD) (C : CmptName)
     (p : Perm) (g : Locality)
-    (b e a : Addr) (cstk : CSTK) (Ws : list WORLD) (Cs : list CmptName) (wstk : Word) (Nswitcher : namespace) :
-    na_inv logrel_nais Nswitcher switcher_inv
+    (b e a : Addr) (cstk : CSTK) (Ws : list WORLD) (Cs : list CmptName) (wstk : Word) :
     ⊢ interp W C (WCap p g b e a) →
       interp_expression cstk Ws Cs W C (WCap p g b e a) wstk.
   Proof.
-    iIntros "#Hswitcher_inv #Hinv_interp".
+    iIntros "#Hinv_interp".
     iIntros (regs) "[[Hfull Hreg] [Hmreg [%Hwstk [Hr [Hsts [Hcont [Hown [Hframe %Hframe]]]]]]]]".
     assert ( readAllowed p = true \/ readAllowed p = false )
       as [Hread_p|Hread_p] by (destruct_perm p ; naive_solver)
@@ -357,12 +354,12 @@ Section fundamental.
       Unshelve. rewrite /persistent_cond in Hperscond_P''; apply _.
   Qed.
 
-  Theorem fundamental W cstk Ws Cs C w wstk Nswitcher :
-    na_inv logrel_nais Nswitcher switcher_inv ⊢ interp W C w -∗ interp_expression cstk Ws Cs W C w wstk.
+  Theorem fundamental W cstk Ws Cs C w wstk :
+    ⊢ interp W C w -∗ interp_expression cstk Ws Cs W C w wstk.
   Proof.
-    iIntros "#Hswitcher Hw". destruct w as [| [c | ] | | ].
+    iIntros "Hw"; destruct w as [| [c | ] | | ].
     2: { iApply fundamental_cap; done. }
-    all: iClear "Hw Hswitcher"; iIntros (?) "(? & Hreg & ?)"; unfold interp_conf.
+    all: iIntros (?) "(? & Hreg & ?)"; unfold interp_conf.
     all: iApply (wp_wand with "[-]"); [ | iIntros (?) "H"; iApply "H"].
     all: iApply (wp_bind (fill [SeqCtx])); cbn.
     all: unfold registers_pointsto; rewrite -insert_delete_insert.
@@ -373,12 +370,11 @@ Section fundamental.
   Qed.
 
   (* The fundamental theorem implies the exec_cond *)
-  Lemma interp_exec_cond W C p g b e a cstk Ws Cs wstk Nswitcher:
+  Lemma interp_exec_cond W C p g b e a cstk Ws Cs wstk:
     executeAllowed p = true ->
-    na_inv logrel_nais Nswitcher switcher_inv ⊢
-    interp W C (WCap p g b e a) -∗ exec_cond W C p g b e cstk Ws Cs wstk interp.
+    ⊢ interp W C (WCap p g b e a) -∗ exec_cond W C p g b e cstk Ws Cs wstk interp.
   Proof.
-    iIntros (Hp) "#Hinv_switcher #Hw".
+    iIntros (Hp) "#Hw".
     iIntros (a0 W' Hin) "#Hfuture". iModIntro.
     assert (isO p = false) by (by eapply executeAllowed_nonO).
     destruct g.
@@ -391,13 +387,12 @@ Section fundamental.
   Qed.
 
   (* We can use the above fact to create a special "jump or fail pattern" when jumping to an unknown adversary *)
-  Lemma exec_wp W C p g b e a cstk Ws Cs wstk Nswitcher :
+  Lemma exec_wp W C p g b e a cstk Ws Cs wstk :
     isCorrectPC (WCap p g b e a) ->
-    na_inv logrel_nais Nswitcher switcher_inv ⊢
-    exec_cond W C p g b e cstk Ws Cs wstk interp -∗
+    ⊢ exec_cond W C p g b e cstk Ws Cs wstk interp -∗
     ∀ W', future_world g W W' → ▷ (interp_expr interp (interp_cont interp cstk Ws Cs) cstk Ws Cs W' C (WCap p g b e a)) wstk.
   Proof.
-    iIntros (Hvpc) "#Hinv_switcher Hexec".
+    iIntros (Hvpc) "Hexec".
     rewrite /exec_cond /enter_cond.
     iIntros (W'). rewrite /future_world.
     assert (a ∈ₐ[[b,e]])%I as Hin.
@@ -411,24 +406,21 @@ Section fundamental.
       iFrame.
   Qed.
 
-  Lemma fundamental_ih Nswitcher :
-    na_inv logrel_nais Nswitcher switcher_inv
+  Lemma fundamental_ih :
     ⊢ ftlr_IH.
   Proof.
-    iIntros "#Hinv".
     iModIntro; iNext.
     iIntros (????????????) "??????????#Hv".
-    iDestruct (fundamental with "[$] Hv") as "Hcont".
+    iDestruct (fundamental with "Hv") as "Hcont".
     iApply "Hcont"; iFrame.
   Qed.
 
   (* updatePcPerm adds a later because of the case of E-capabilities, which *)
   (*    unfold to ▷ interp_expr *)
-  Lemma interp_updatePcPerm W C w Nswitcher :
-    na_inv logrel_nais Nswitcher switcher_inv
+  Lemma interp_updatePcPerm W C w :
     ⊢ interp W C w -∗ ▷ (∀ cstk Ws Cs wstk, interp_expression cstk Ws Cs W C (updatePcPerm w) wstk).
   Proof.
-    iIntros "#Hswitcher #Hw".
+    iIntros "#Hw".
     assert ( ( (∃ p g b e a, w = WSentry p g b e a))
             ∨ updatePcPerm w = w)
       as [ Hw | ->].
@@ -447,8 +439,8 @@ Section fundamental.
     { iNext; iIntros (????); iApply fundamental; eauto. }
   Qed.
 
-  Lemma jmp_or_fail_spec W C w φ cstk Ws Cs wstk Nswitcher :
-    na_inv logrel_nais Nswitcher switcher_inv ⊢
+  Lemma jmp_or_fail_spec W C w φ cstk Ws Cs wstk :
+    ⊢
     (interp W C w
      -∗ (if decide (isCorrectPC (updatePcPerm w))
          then
@@ -459,14 +451,14 @@ Section fundamental.
          else φ FailedV ∗ PC ↦ᵣ updatePcPerm w
                           -∗ WP Seq (Instr Executable) {{ φ }} )).
   Proof.
-    iIntros "#Hinv_switcher #Hw".
+    iIntros "#Hw".
     destruct (decide (isCorrectPC (updatePcPerm w))).
     - inversion i.
       destruct w;inv H.
       + destruct p; cbn in * ; simplify_eq.
         iExists _,_,_,_,_.
         iSplit;[eauto|]. iModIntro.
-        iDestruct (interp_exec_cond with "[$] [$Hw]") as "Hexec";[auto|].
+        iDestruct (interp_exec_cond with "[$Hw]") as "Hexec";[auto|].
         iApply exec_wp;auto.
       + destruct p0; cbn in * ; simplify_eq.
         iExists _,_,_,_,_.
