theories/logrel/logrel_extra.v
@@ -16,7 +16,6 @@ Section Logrel_extra.
     {stsg : STSG Addr region_type Σ} {cstackg : CSTACKG Σ} {heapg : heapGS Σ}
     {nainv: logrel_na_invs Σ}
     `{MP: MachineParameters}
-    {swlayout : switcherLayout}
   .
 
   Implicit Types W : WORLD.
